renaming tac effect combinators

ulib/FStar.Tactics.Effect.fst
@@ -19,6 +19,11 @@ open FStar.Reflection.Types
 open FStar.Tactics.Types
 open FStar.Tactics.Result
 
+#push-options "--admit_smt_queries true"
+let tac_bind_interleave_begin = ()
+#pop-options
+let tac_bind_interleave_end = ()
+
 let with_tactic _ p = p
 
 let rewrite_with_tactic _ p = p
